src/PlutusIR/Semantics/Static/Typing/Typechecker.v
@@ -1,0 +1,216 @@
+
+Require Import Coq.Lists.List.
+Import ListNotations.
+Require Import Coq.Bool.Bool.
+Require Import Coq.Strings.String.
+
+Local Open Scope string_scope.
+
+From PlutusCert Require Import 
+    Normalisation.Normalisation 
+    Normalisation.Normaliser_sound_complete
+    Normalisation.Normaliser
+    PlutusIR 
+    Static.Typing.Typing
+    Util.List
+    Static.Util
+    Equality
+    Kinding.Checker
+    Util
+    SubstituteTCA
+    UniqueTypes
+    Typing.Binders_Wellkinded
+    BaseKindedness.
+Require Import PlutusCert.PlutusIR.Analysis.BoundVars.
+
+From Coq Require Import Program.Equality.
+
+(* Find instead of in_dec for performance?*)
+Fixpoint no_dup_fun (xs : list string) := 
+  match xs with
+  | nil => true
+  | (x::xs) => if in_dec string_dec x xs then false else no_dup_fun xs
+  end.
+
+
+Definition is_KindBase (k : option kind) : bool :=
+  match k with 
+  | Some Kind_Base => true
+  | _ => false
+  end.
+
+Definition constructor_well_formed_check (Δ : list (binderTyname * kind)) (v : vdecl) (Tr : ty ) : bool :=
+  match v with
+  | VarDecl x T => let (targs, tr') := splitTy T in
+          Ty_eqb Tr tr' && forallb (fun U => is_KindBase (kind_check Δ U)) targs
+  end.
+
+(* Idea Jacco: pass the recursively called type_check function as an argument even though it is not defined yet 
+Make another version that already has type_check as argument after type_check is defined.
+*)
+Definition binding_well_formed_check 
+  (type_check' : ((list (binderTyname * kind)) -> (list (binderName * ty)) -> term -> option ty)) 
+  (Δ : list (binderTyname * kind)) (Γ : list (binderName * ty)) (rec : recursivity) binding : bool :=
+    match binding with
+    | (TypeBind (TyVarDecl X K) T) => match kind_check Δ T with
+                                      | Some K' => Kind_eqb K K' (* is this K the same as in the pattern match to the left? it should be*)
+                                      | _ => false
+                                      end
+    | (TermBind s (VarDecl x T) t) => match kind_check Δ T with
+                                      | Some Kind_Base => 
+                                        match type_check' Δ Γ t with   
+                                        | Some Tn => match normaliser Δ T with
+                                                    | Some Tn' => Ty_eqb Tn Tn'
+                                                    | _ => false
+                                                    end
+                                        | _ => false
+                                        end
+                                      | _ => false
+                                      end
+    | (DatatypeBind (Datatype XK YKs matchFunc cs)) => 
+      let dtd := Datatype XK YKs matchFunc cs in
+      let X := tvdecl_name XK in
+      let Ys := map tvdecl_name YKs in
+      if no_dup_fun (X :: Ys) && no_dup_fun (map vdecl_name cs) then
+        let Δ_ns := match rec with
+                    | NonRec => drop_Δ' Δ [X]
+                    | Rec => Δ
+                    end in
+        let Δ' := rev (map fromDecl YKs) ++ Δ_ns in
+        let Tres := constrLastTyExpected dtd in
+        if forallb (fun c => constructor_well_formed_check Δ' c Tres) cs then
+          match rec with
+            | NonRec => match kind_check (fromDecl XK :: Δ') Tres with
+                        | Some Kind_Base => true 
+                        | _ => false
+                        end
+            | Rec =>    match kind_check Δ' Tres with
+                        | Some Kind_Base => true 
+                        | _ => false  
+                        end
+          end
+        else false
+      else false
+    end.
+
+(* first argument represents binding_well_formed with the type_check already passed in *)
+Definition bindings_well_formed_nonrec_check : 
+  ((list (binderTyname * kind)) -> (list (binderName * ty)) -> recursivity -> binding -> bool) ->
+  list (binderTyname * kind) -> (list (binderName * ty)) -> (list binding) -> bool :=
+  fun b_wf =>
+  fix f Δ Γ bs :=
+    match bs with
+      | (b::bs') =>
+            match (map_normaliser (insert_deltas_rec (binds_Gamma b) (binds_Delta b ++ Δ))) with
+            | Some bsGn =>
+              b_wf Δ Γ NonRec b && f ((binds_Delta b) ++ Δ) (bsGn ++ Γ) bs'
+            | _ => false
+            end
+      | _ => true
+    end.
+
+Definition bindings_well_formed_rec_check : (binding -> bool) -> list binding -> bool :=
+  fun b_wf =>
+  fix f bs :=
+    match bs with
+      | (b::bs') => b_wf b && f bs'
+      | _ => true
+    end.
+
+Fixpoint type_check (Δ : list (binderTyname * kind)) (Γ : list (binderName * ty)) (term : term) {struct term} : (option ty) :=
+    match term with
+    | Var x => lookup x Γ >>= fun T => 
+                match kind_check Δ T with
+                | Some Kind_Base => normaliser Δ T
+                | _ => None
+                end
+    | LamAbs x T1 t => 
+        normaliser Δ T1 >>= fun T1n =>
+        match type_check Δ ((x, T1n) :: Γ) t, kind_check Δ T1 with
+        | Some T2, Some Kind_Base => Some (Ty_Fun T1n T2) 
+        | _, _ => None
+        end
+    | Apply t1 t2 => 
+        match type_check Δ Γ t1, type_check Δ Γ t2 with
+        | Some (Ty_Fun T1 T2), Some T1' =>
+            if Ty_eqb T1 T1' then Some T2 else None
+        | _, _ => None
+        end
+    | TyAbs X K t => 
+        match type_check ((X, K) :: Δ) (drop_ty_var X Γ) t with
+        | Some T => Some (Ty_Forall X K T)
+        | _ => None
+        end
+    | TyInst t1 T2 => 
+        match type_check Δ Γ t1, kind_check Δ T2 with
+        | Some (Ty_Forall X K2 T1), Some K2' =>
+            if Kind_eqb K2 K2' then 
+                normaliser Δ T2 >>= fun T2n =>
+                normaliser Δ (substituteTCA X T2n T1) >>= fun T0n =>
+                Some T0n
+            else None
+        | _, _ => None
+        end
+    | IWrap F T M =>
+        match kind_check Δ T, kind_check Δ F, type_check Δ Γ M with
+        | Some K, Some (Kind_Arrow (Kind_Arrow K' Kind_Base) (Kind_Arrow K'' Kind_Base)), Some T0n
+            => if andb (Kind_eqb K K') (Kind_eqb K K'') then
+                    normaliser Δ T >>= fun Tn =>
+                    normaliser Δ F >>= fun Fn =>
+                    normaliser Δ (unwrapIFix Fn K Tn) >>= fun T0n' =>
+                    if Ty_eqb T0n T0n' then 
+                        Some (Ty_IFix Fn Tn)
+                    else None 
+                else None 
+        | _, _, _ => None
+        end
+    | Unwrap M =>
+        match type_check Δ Γ M with
+            | Some (Ty_IFix F T) =>
+                match kind_check Δ T with
+                    | Some K =>
+                          normaliser Δ (unwrapIFix F K T) >>= fun T0n => Some T0n
+                        
+                    | _  => None
+                    end 
+            | _ => None
+            end
+    | Constant (ValueOf T a) => Some (Ty_Builtin T)
+    | Builtin f =>
+        let T := lookupBuiltinTy f in
+        normaliser Δ T >>= fun Tn =>
+        Some Tn
+    | Error S' => normaliser Δ S' >>= fun S'n => match kind_check Δ S' with
+        | Some Kind_Base => Some S'n
+        | _ => None
+        end
+    | Let NonRec bs t =>
+        let Δ' := flatten (map binds_Delta bs) ++ Δ in
+        let xs := (insert_deltas_bind_Gamma_nr bs Δ) in
+          map_normaliser xs >>= fun bsgn => 
+          let Γ' := bsgn ++ Γ in
+          if (bindings_well_formed_nonrec_check (binding_well_formed_check type_check) Δ Γ bs) then 
+            type_check Δ' Γ' t >>= fun T =>
+              let Δ_no_esc := drop_Δ Δ bs in
+              match kind_check Δ_no_esc T with
+              | Some Kind_Base => Some T
+              | _ => None
+              end
+          else None
+    | Let Rec bs t => 
+        if no_dup_fun (btvbs bs) && no_dup_fun (bvbs bs) then
+          let Δ' := flatten (map binds_Delta bs) ++ Δ in
+          let xs := (insert_deltas_rec (flatten (map binds_Gamma bs)) Δ') in
+            map_normaliser xs >>= fun bsgn =>
+            let Γ' := bsgn ++ Γ in
+              if (bindings_well_formed_rec_check (binding_well_formed_check type_check Δ' Γ' Rec) bs) then 
+                type_check Δ' Γ' t >>= fun T =>
+                  let Δ_no_esc := drop_Δ Δ bs in
+                  match kind_check Δ_no_esc T with
+                  | Some Kind_Base => Some T
+                  | _ => None
+                    end 
+              else None
+          else None
+    | _ => None (* TODO: Case and Constr?? *)
+    end.
